### 1. Identity Law
- **OR Form**: \( P + 0 = P \) (Adding zero to a value does not change the value)
- **AND Form**: \( P \cdot 1 = P \) (Multiplying a value by one does not change the value)

### 2. Idempotent Law
- **OR Form**: \( P + P = P \) (Adding a value to itself does not change the value)
- **AND Form**: \( P \cdot P = P \) (Multiplying a value by itself does not change the value)

### 3. Commutative Law
- **OR Form**: \( P + Q = Q + P \) (The order of addition does not matter)
- **AND Form**: \( P \cdot Q = Q \cdot P \) (The order of multiplication does not matter)

### 4. Associative Law
- **OR Form**: \( P + (Q + R) = (P + Q) + R \) (Grouping does not affect the result of addition)
- **AND Form**: \( P \cdot (Q \cdot R) = (P \cdot Q) \cdot R \) (Grouping does not affect the result of multiplication)

### 5. Distributive Law
- **OR Form**: \( P + (Q \cdot R) = (P + Q) \cdot (P + R) \) (Distributing addition over multiplication)
- **AND Form**: \( P \cdot (Q + R) = (P \cdot Q) + (P \cdot R) \) (Distributing multiplication over addition)

### 6. Inversion Law
- **Both Forms**: \( (A')' = A \) (The double negation of a value returns the original value)

### 7. De Morgan's Law
- **OR Form**: \( (P + Q)' = P' \cdot Q' \) (The negation of a sum is the product of the negations)
- **AND Form**: \( (P \cdot Q)' = P' + Q' \) (The negation of a product is the sum of the negations)

### 8. Complement Law
- **OR Form**: \( P + P' = 1 \) (A value ORed with its complement equals true)
- **AND Form**: \( P \cdot P' = 0 \) (A value ANDed with its complement equals false)

### 9. Domination Law
- **OR Form**: \( P + 1 = 1 \) (A value ORed with true equals true)
- **AND Form**: \( P \cdot 0 = 0 \) (A value ANDed with false equals false)

### 10. Double Negation Law
- **Both Forms**: \( (P')' = P \) (The double negation of a value returns the original value)

### 11. Absorption Law
- **OR Form**: \( P + (P \cdot Q) = P \) (A value ORed with the product of itself and another value equals the original value)
- **AND Form**: \( P \cdot (P + Q) = P \) (A value ANDed with the sum of itself and another value equals the original value)

source: https://www.geeksforgeeks.org/boolean-algebra/